query bounding complexity

VCVio/OracleComp/QueryBound.lean
@@ -26,8 +26,14 @@ variable {ι : Type} [DecidableEq ι] {spec : OracleSpec ι} {α β γ : Type}
 def IsQueryBound (oa : OracleComp spec α) (qb : ι → ℕ) : Prop :=
     ∀ qc ∈ (snd <$> simulate countingOracle 0 oa).support, qc ≤ qb
 
-lemma isQueryBound_def (oa : OracleComp spec α) (qb : ι → ℕ) : IsQueryBound oa qb ↔
-    ∀ qc ∈ (snd <$> simulate countingOracle 0 oa).support, qc ≤ qb := Iff.rfl
+lemma isQueryBound_def (oa : OracleComp spec α) (qb : ι → ℕ) :
+    IsQueryBound oa qb ↔ ∀ qc ∈ (snd <$> simulate countingOracle 0 oa).support, qc ≤ qb := Iff.rfl
+
+lemma isQueryBound_mono {oa : OracleComp spec α} {qb qb' : ι → ℕ}
+    (h' : IsQueryBound oa qb) (h : qb ≤ qb') : IsQueryBound oa qb' := by
+  intro qc hqc
+  specialize h' qc hqc
+  refine le_trans h' h
 
 @[simp]
 lemma isQueryBound_pure (a : α) (qb : ι → ℕ) :
@@ -36,15 +42,24 @@ lemma isQueryBound_pure (a : α) (qb : ι → ℕ) :
 
 @[simp]
 lemma isQueryBound_query_iff (i : ι) (t : spec.domain i) (qb : ι → ℕ) :
-    IsQueryBound (query i t) qb ↔ 0 < qb i := by
-  simp [isQueryBound_def, Nat.lt_iff_add_one_le, zero_add]
+    IsQueryBound (query i t) qb ↔ qb i ≠ 0 := by
+  simp [isQueryBound_def, Nat.lt_iff_add_one_le, zero_add, ← Nat.pos_iff_ne_zero]
   refine ⟨λ h ↦ le_of_eq_of_le (symm <| Function.update_same i 1 0) (h i), λ h j ↦ ?_⟩
   by_cases hij : j = i
   · induction hij
     simpa using h
   · simp [Function.update_noteq hij]
 
-lemma isQueryBound_bind (oa : OracleComp spec α) (ob : α → OracleComp spec β) (qb₁ qb₂ : ι → ℕ)
+lemma isQueryBound_query (i : ι) (t : spec.domain i) {qb : ι → ℕ} (hqb : qb i ≠ 0) :
+    IsQueryBound (query i t) qb :=
+  (isQueryBound_query_iff i t qb).2 hqb
+
+lemma update_isQueryBound_query (i : ι) (t : spec.domain i) :
+    IsQueryBound (query i t) (Function.update 0 i 1) := by
+  refine isQueryBound_query i t ?_
+  simp only [Function.update_same, ne_eq, one_ne_zero, not_false_eq_true]
+
+lemma isQueryBound_bind {oa : OracleComp spec α} {ob : α → OracleComp spec β} {qb₁ qb₂ : ι → ℕ}
     (h1 : IsQueryBound oa qb₁) (h2 : ∀ x, IsQueryBound (ob x) qb₂) :
     IsQueryBound (oa >>= ob) (qb₁ + qb₂) := by
   intros count h
@@ -52,9 +67,14 @@ lemma isQueryBound_bind (oa : OracleComp spec α) (ob : α → OracleComp spec �
   obtain ⟨y, x, count', h, h'⟩ := h
   specialize h1 count'
   rw [support_map] at h1
-  have : count' ≤ count := sorry
+  have : count' ≤ count :=
+    countingOracle.le_of_mem_support_simulate (ob x) _ _ y h'
   specialize h1 ⟨⟨x, count'⟩, h, rfl⟩
-  specialize h2 x (count - count') sorry
+  specialize h2 x (count - count') (by {
+    rw [← countingOracle.mem_support_snd_map_simulate_iff_of_le _ this,
+      support_map, Set.mem_image] -- TODO: shouldn't need two steps
+    refine ⟨(y, count), h', rfl⟩
+  })
   have h3 := add_le_add h2 h1
   rw [add_comm qb₂] at h3
   refine le_trans ?_ h3
@@ -63,10 +83,128 @@ lemma isQueryBound_bind (oa : OracleComp spec α) (ob : α → OracleComp spec �
   simp only [Pi.add_apply, Pi.sub_apply]
   rw [tsub_add_cancel_of_le this]
 
+section minimalQueryBound
+
+/-- The minimal query bound on a computation. Note that this is noncomputatble,
+since we need to take a minimum over the entire codomain at each query step. -/
+def minimalQueryBound : {α : Type} → OracleComp spec α → (ι → ℕ)
+  | _, pure' _ _ => 0
+  | _, queryBind' i _ _ oa => λ j ↦ (if j = i then 1 else 0) +
+      (Finset.max' (Finset.univ.image <| λ u ↦ minimalQueryBound (oa u) j)
+        (by simpa using Finset.univ_nonempty))
+
+lemma isQueryBound_minimalQueryBound (oa : OracleComp spec α) :
+    IsQueryBound oa (minimalQueryBound oa) := by
+  induction oa using OracleComp.inductionOn with
+  | h_pure x => exact isQueryBound_pure x _
+  | h_queryBind i t oa hoa =>
+    · refine isQueryBound_bind (by simp) <| λ u ↦ isQueryBound_mono (hoa u)
+        (λ j ↦ Finset.le_max' _ _ ?_)
+      simp only [OracleComp.bind'_eq_bind, pure_bind, Finset.mem_image, Finset.mem_univ, true_and,
+        exists_apply_eq_apply]
+
+lemma minimalQueryBound_mem_support_simulate (oa : OracleComp spec α) :
+    minimalQueryBound oa ∈ (snd <$> simulate countingOracle 0 oa).support := by
+  induction oa using OracleComp.inductionOn with
+  | h_pure x => rfl
+  | h_queryBind i t oa hoa => {
+    simp only [minimalQueryBound]
+    sorry
+  }
+
+lemma minimalQueryBound_minimal (oa : OracleComp spec α) :
+    Minimal (IsQueryBound oa) (minimalQueryBound oa) := by
+  rw [minimal_iff]
+  refine ⟨isQueryBound_minimalQueryBound oa, ?_⟩
+  sorry
+
+lemma le_minimalQueryBound_of_isQueryBound {oa : OracleComp spec α} (qc : ι → ℕ)
+    (hqc : IsQueryBound oa qc) : minimalQueryBound oa ≤ qc := by
+  induction oa using OracleComp.inductionOn with
+  | h_pure x => {
+    exact zero_le _
+  }
+  | h_queryBind i t oa hoa => {
+    simp only [minimalQueryBound]
+    intro j
+    by_cases hj : j = i
+    · induction hj
+      simp
+      sorry
+    · simp [hj]
+      sorry
+  }
+
+lemma exists_isQueryBound (oa : OracleComp spec α) : ∃ qc, IsQueryBound oa qc :=
+  ⟨minimalQueryBound oa, isQueryBound_minimalQueryBound oa⟩
+
+lemma exists_minimal_isQueryBound (oa : OracleComp spec α) :
+    ∃ qc, IsQueryBound oa qc ∧ (∀ qc', IsQueryBound oa qc' → qc ≤ qc') := by
+  refine ⟨minimalQueryBound oa, isQueryBound_minimalQueryBound oa,
+    le_minimalQueryBound_of_isQueryBound⟩
+
+end minimalQueryBound
+
+lemma isQueryBound_query_bind_iff (i : ι) (t : spec.domain i)
+    (oa : spec.range i → OracleComp spec α) (qc : ι → ℕ) :
+    IsQueryBound (query i t >>= oa) qc ↔ qc i ≠ 0 ∧
+      ∀ u, IsQueryBound (oa u) (Function.update qc i (qc i - 1)) := by
+  refine ⟨λ h ↦ ⟨?_, ?_⟩, λ h ↦ ?_⟩
+  ·
+    specialize h (minimalQueryBound (query i t >>= oa))
+    sorry
+  · sorry
+  · refine isQueryBound_mono (isQueryBound_bind (update_isQueryBound_query i t) h.2) ?_
+    intro j
+    by_cases hj : j = i
+    · simp only [hj, Pi.add_apply, Function.update_same]
+      rw [Nat.add_sub_of_le]
+      rw [Nat.one_le_iff_ne_zero]
+      exact h.1
+    · simp [hj]
+
 @[simp]
 lemma isQueryBound_map_iff (oa : OracleComp spec α) (f : α → β) (qb : ι → ℕ) :
     IsQueryBound (f <$> oa) qb ↔ IsQueryBound oa qb := by
   simp [isQueryBound_def]
+
+-- isQueryBound_seq_iff
+
+section simulate
+
+variable {ι' : Type} {spec' : OracleSpec ι} {σ : Type}
+
+/-- If we have a query bound on a computation, and a query bound on a `SimOracle` implementation,
+then their product is a query bound on the -/
+lemma isQueryBound_simulate (oa : OracleComp spec α) (so : spec →[σ]ₛₒ spec') (s : σ)
+    {qb qbs : ι → ℕ} (hqb : IsQueryBound oa qb) (hqbs : ∀ i t s, IsQueryBound (so i t s) qbs) :
+    IsQueryBound (simulate so s oa) (qb * qbs) := by
+  induction oa using OracleComp.inductionOn with
+  | h_pure x => exact isQueryBound_pure (x, s) (qb * qbs)
+  | h_queryBind i t oa hoa => {
+      rw [simulate_query_bind]
+      sorry
+  }
+
+end simulate
+
+
+-- @[simp] -- TODO: isPure predicate?
+-- lemma zero_isQueryBound_iff (oa : OracleComp spec α) :
+--     IsQueryBound oa 0 ↔ ∃ x, oa = pure x := by
+--   refine ⟨λ h ↦ ?_, λ ⟨x, hx⟩ ↦ hx ▸ isQueryBound_pure x 0⟩
+--   induction oa using OracleComp.inductionOn with
+--   | h_pure x => exact ⟨x, rfl⟩
+--   | h_queryBind i t oa hoa => {
+--     simp
+--     specialize h (minimalQueryBound (query i t >>= oa)) ?_
+--     ·
+--       sorry
+--     · specialize h i
+--       simp [minimalQueryBound] at h
+
+
+--   }
 
 end IsQueryBound
 
